AwsCryptographicMaterialProviders/runtimes/java/src/main/smithy-generated/software/amazon/cryptography/keystoreadmin/model/KmsAes.java
@@ -1,0 +1,98 @@
+// Copyright Amazon.com Inc. or its affiliates. All Rights Reserved.
+// SPDX-License-Identifier: Apache-2.0
+// Do not modify this file. This file is machine generated, and any changes to it will be overwritten.
+package software.amazon.cryptography.keystoreadmin.model;
+
+import java.util.Objects;
+import software.amazon.cryptography.keystore.model.AwsKms;
+
+/**
+ * Include all attributes of an item as Encryption Context
+ * in a KMS Encrypt or Decrypt call,
+ * effectively signing the attributes.
+ */
+public class KmsAes {
+
+  private final KmsAesIdentifier KmsAesIdentifier;
+
+  private final AwsKms AwsKms;
+
+  protected KmsAes(BuilderImpl builder) {
+    this.KmsAesIdentifier = builder.KmsAesIdentifier();
+    this.AwsKms = builder.AwsKms();
+  }
+
+  public KmsAesIdentifier KmsAesIdentifier() {
+    return this.KmsAesIdentifier;
+  }
+
+  public AwsKms AwsKms() {
+    return this.AwsKms;
+  }
+
+  public Builder toBuilder() {
+    return new BuilderImpl(this);
+  }
+
+  public static Builder builder() {
+    return new BuilderImpl();
+  }
+
+  public interface Builder {
+    Builder KmsAesIdentifier(KmsAesIdentifier KmsAesIdentifier);
+
+    KmsAesIdentifier KmsAesIdentifier();
+
+    Builder AwsKms(AwsKms AwsKms);
+
+    AwsKms AwsKms();
+
+    KmsAes build();
+  }
+
+  static class BuilderImpl implements Builder {
+
+    protected KmsAesIdentifier KmsAesIdentifier;
+
+    protected AwsKms AwsKms;
+
+    protected BuilderImpl() {}
+
+    protected BuilderImpl(KmsAes model) {
+      this.KmsAesIdentifier = model.KmsAesIdentifier();
+      this.AwsKms = model.AwsKms();
+    }
+
+    public Builder KmsAesIdentifier(KmsAesIdentifier KmsAesIdentifier) {
+      this.KmsAesIdentifier = KmsAesIdentifier;
+      return this;
+    }
+
+    public KmsAesIdentifier KmsAesIdentifier() {
+      return this.KmsAesIdentifier;
+    }
+
+    public Builder AwsKms(AwsKms AwsKms) {
+      this.AwsKms = AwsKms;
+      return this;
+    }
+
+    public AwsKms AwsKms() {
+      return this.AwsKms;
+    }
+
+    public KmsAes build() {
+      if (Objects.isNull(this.KmsAesIdentifier())) {
+        throw new IllegalArgumentException(
+          "Missing value for required field `KmsAesIdentifier`"
+        );
+      }
+      if (Objects.isNull(this.AwsKms())) {
+        throw new IllegalArgumentException(
+          "Missing value for required field `AwsKms`"
+        );
+      }
+      return new KmsAes(this);
+    }
+  }
+}
