AwsCryptographicMaterialProviders/runtimes/net/Generated/AwsCryptographyKeyStore/MutationIndex.cs
@@ -1,0 +1,70 @@
+// Copyright Amazon.com Inc. or its affiliates. All Rights Reserved.
+// SPDX-License-Identifier: Apache-2.0
+// Do not modify this file. This file is machine generated, and any changes to it will be overwritten.
+using System;
+using AWS.Cryptography.KeyStore;
+namespace AWS.Cryptography.KeyStore
+{
+  public class MutationIndex
+  {
+    private string _identifier;
+    private string _createTime;
+    private string _uUID;
+    private System.IO.MemoryStream _pageIndex;
+    private System.IO.MemoryStream _enc;
+    public string Identifier
+    {
+      get { return this._identifier; }
+      set { this._identifier = value; }
+    }
+    public bool IsSetIdentifier()
+    {
+      return this._identifier != null;
+    }
+    public string CreateTime
+    {
+      get { return this._createTime; }
+      set { this._createTime = value; }
+    }
+    public bool IsSetCreateTime()
+    {
+      return this._createTime != null;
+    }
+    public string UUID
+    {
+      get { return this._uUID; }
+      set { this._uUID = value; }
+    }
+    public bool IsSetUUID()
+    {
+      return this._uUID != null;
+    }
+    public System.IO.MemoryStream PageIndex
+    {
+      get { return this._pageIndex; }
+      set { this._pageIndex = value; }
+    }
+    public bool IsSetPageIndex()
+    {
+      return this._pageIndex != null;
+    }
+    public System.IO.MemoryStream Enc
+    {
+      get { return this._enc; }
+      set { this._enc = value; }
+    }
+    public bool IsSetEnc()
+    {
+      return this._enc != null;
+    }
+    public void Validate()
+    {
+      if (!IsSetIdentifier()) throw new System.ArgumentException("Missing value for required property 'Identifier'");
+      if (!IsSetCreateTime()) throw new System.ArgumentException("Missing value for required property 'CreateTime'");
+      if (!IsSetUUID()) throw new System.ArgumentException("Missing value for required property 'UUID'");
+      if (!IsSetPageIndex()) throw new System.ArgumentException("Missing value for required property 'PageIndex'");
+      if (!IsSetEnc()) throw new System.ArgumentException("Missing value for required property 'Enc'");
+
+    }
+  }
+}
