AwsCryptographicMaterialProviders/runtimes/net/Generated/AwsCryptographyKeyStore/TypeConversion.cs
@@ -24,26 +24,6 @@ namespace AWS.Cryptography.KeyStore
       ToDafny_N3_aws__N12_cryptography__N8_keyStore__S28_AlreadyExistsConditionFailed__M7_message(value.Message)
       );
     }
-    public static AWS.Cryptography.KeyStore.ClobberMutationLockInput FromDafny_N3_aws__N12_cryptography__N8_keyStore__S24_ClobberMutationLockInput(software.amazon.cryptography.keystore.internaldafny.types._IClobberMutationLockInput value)
-    {
-      software.amazon.cryptography.keystore.internaldafny.types.ClobberMutationLockInput concrete = (software.amazon.cryptography.keystore.internaldafny.types.ClobberMutationLockInput)value; AWS.Cryptography.KeyStore.ClobberMutationLockInput converted = new AWS.Cryptography.KeyStore.ClobberMutationLockInput(); converted.MutationLock = (AWS.Cryptography.KeyStore.MutationLock)FromDafny_N3_aws__N12_cryptography__N8_keyStore__S24_ClobberMutationLockInput__M12_MutationLock(concrete._MutationLock); return converted;
-    }
-    public static software.amazon.cryptography.keystore.internaldafny.types._IClobberMutationLockInput ToDafny_N3_aws__N12_cryptography__N8_keyStore__S24_ClobberMutationLockInput(AWS.Cryptography.KeyStore.ClobberMutationLockInput value)
-    {
-      value.Validate();
-
-      return new software.amazon.cryptography.keystore.internaldafny.types.ClobberMutationLockInput(ToDafny_N3_aws__N12_cryptography__N8_keyStore__S24_ClobberMutationLockInput__M12_MutationLock(value.MutationLock));
-    }
-    public static AWS.Cryptography.KeyStore.ClobberMutationLockOutput FromDafny_N3_aws__N12_cryptography__N8_keyStore__S25_ClobberMutationLockOutput(software.amazon.cryptography.keystore.internaldafny.types._IClobberMutationLockOutput value)
-    {
-      software.amazon.cryptography.keystore.internaldafny.types.ClobberMutationLockOutput concrete = (software.amazon.cryptography.keystore.internaldafny.types.ClobberMutationLockOutput)value; AWS.Cryptography.KeyStore.ClobberMutationLockOutput converted = new AWS.Cryptography.KeyStore.ClobberMutationLockOutput(); return converted;
-    }
-    public static software.amazon.cryptography.keystore.internaldafny.types._IClobberMutationLockOutput ToDafny_N3_aws__N12_cryptography__N8_keyStore__S25_ClobberMutationLockOutput(AWS.Cryptography.KeyStore.ClobberMutationLockOutput value)
-    {
-      value.Validate();
-
-      return new software.amazon.cryptography.keystore.internaldafny.types.ClobberMutationLockOutput();
-    }
     public static AWS.Cryptography.KeyStore.CreateKeyInput FromDafny_N3_aws__N12_cryptography__N8_keyStore__S14_CreateKeyInput(software.amazon.cryptography.keystore.internaldafny.types._ICreateKeyInput value)
     {
       software.amazon.cryptography.keystore.internaldafny.types.CreateKeyInput concrete = (software.amazon.cryptography.keystore.internaldafny.types.CreateKeyInput)value; AWS.Cryptography.KeyStore.CreateKeyInput converted = new AWS.Cryptography.KeyStore.CreateKeyInput(); if (concrete._branchKeyIdentifier.is_Some) converted.BranchKeyIdentifier = (string)FromDafny_N3_aws__N12_cryptography__N8_keyStore__S14_CreateKeyInput__M19_branchKeyIdentifier(concrete._branchKeyIdentifier);
@@ -85,6 +65,26 @@ namespace AWS.Cryptography.KeyStore
       value.Validate();
 
       return new software.amazon.cryptography.keystore.internaldafny.types.CreateKeyStoreOutput(ToDafny_N3_aws__N12_cryptography__N8_keyStore__S20_CreateKeyStoreOutput__M8_tableArn(value.TableArn));
+    }
+    public static AWS.Cryptography.KeyStore.DeleteMutationLockAndIndexInput FromDafny_N3_aws__N12_cryptography__N8_keyStore__S31_DeleteMutationLockAndIndexInput(software.amazon.cryptography.keystore.internaldafny.types._IDeleteMutationLockAndIndexInput value)
+    {
+      software.amazon.cryptography.keystore.internaldafny.types.DeleteMutationLockAndIndexInput concrete = (software.amazon.cryptography.keystore.internaldafny.types.DeleteMutationLockAndIndexInput)value; AWS.Cryptography.KeyStore.DeleteMutationLockAndIndexInput converted = new AWS.Cryptography.KeyStore.DeleteMutationLockAndIndexInput(); converted.MutationLock = (AWS.Cryptography.KeyStore.MutationLock)FromDafny_N3_aws__N12_cryptography__N8_keyStore__S31_DeleteMutationLockAndIndexInput__M12_MutationLock(concrete._MutationLock); return converted;
+    }
+    public static software.amazon.cryptography.keystore.internaldafny.types._IDeleteMutationLockAndIndexInput ToDafny_N3_aws__N12_cryptography__N8_keyStore__S31_DeleteMutationLockAndIndexInput(AWS.Cryptography.KeyStore.DeleteMutationLockAndIndexInput value)
+    {
+      value.Validate();
+
+      return new software.amazon.cryptography.keystore.internaldafny.types.DeleteMutationLockAndIndexInput(ToDafny_N3_aws__N12_cryptography__N8_keyStore__S31_DeleteMutationLockAndIndexInput__M12_MutationLock(value.MutationLock));
+    }
+    public static AWS.Cryptography.KeyStore.DeleteMutationLockAndIndexOutput FromDafny_N3_aws__N12_cryptography__N8_keyStore__S32_DeleteMutationLockAndIndexOutput(software.amazon.cryptography.keystore.internaldafny.types._IDeleteMutationLockAndIndexOutput value)
+    {
+      software.amazon.cryptography.keystore.internaldafny.types.DeleteMutationLockAndIndexOutput concrete = (software.amazon.cryptography.keystore.internaldafny.types.DeleteMutationLockAndIndexOutput)value; AWS.Cryptography.KeyStore.DeleteMutationLockAndIndexOutput converted = new AWS.Cryptography.KeyStore.DeleteMutationLockAndIndexOutput(); return converted;
+    }
+    public static software.amazon.cryptography.keystore.internaldafny.types._IDeleteMutationLockAndIndexOutput ToDafny_N3_aws__N12_cryptography__N8_keyStore__S32_DeleteMutationLockAndIndexOutput(AWS.Cryptography.KeyStore.DeleteMutationLockAndIndexOutput value)
+    {
+      value.Validate();
+
+      return new software.amazon.cryptography.keystore.internaldafny.types.DeleteMutationLockAndIndexOutput();
     }
     public static AWS.Cryptography.KeyStore.GetActiveBranchKeyInput FromDafny_N3_aws__N12_cryptography__N8_keyStore__S23_GetActiveBranchKeyInput(software.amazon.cryptography.keystore.internaldafny.types._IGetActiveBranchKeyInput value)
     {
@@ -222,13 +222,15 @@ namespace AWS.Cryptography.KeyStore
     {
       software.amazon.cryptography.keystore.internaldafny.types.GetItemsForInitializeMutationOutput concrete = (software.amazon.cryptography.keystore.internaldafny.types.GetItemsForInitializeMutationOutput)value; AWS.Cryptography.KeyStore.GetItemsForInitializeMutationOutput converted = new AWS.Cryptography.KeyStore.GetItemsForInitializeMutationOutput(); converted.ActiveItem = (AWS.Cryptography.KeyStore.EncryptedHierarchicalKey)FromDafny_N3_aws__N12_cryptography__N8_keyStore__S35_GetItemsForInitializeMutationOutput__M10_ActiveItem(concrete._ActiveItem);
       converted.BeaconItem = (AWS.Cryptography.KeyStore.EncryptedHierarchicalKey)FromDafny_N3_aws__N12_cryptography__N8_keyStore__S35_GetItemsForInitializeMutationOutput__M10_BeaconItem(concrete._BeaconItem);
-      if (concrete._MutationLock.is_Some) converted.MutationLock = (AWS.Cryptography.KeyStore.MutationLock)FromDafny_N3_aws__N12_cryptography__N8_keyStore__S35_GetItemsForInitializeMutationOutput__M12_MutationLock(concrete._MutationLock); return converted;
+      if (concrete._MutationLock.is_Some) converted.MutationLock = (AWS.Cryptography.KeyStore.MutationLock)FromDafny_N3_aws__N12_cryptography__N8_keyStore__S35_GetItemsForInitializeMutationOutput__M12_MutationLock(concrete._MutationLock);
+      if (concrete._MutationIndex.is_Some) converted.MutationIndex = (AWS.Cryptography.KeyStore.MutationIndex)FromDafny_N3_aws__N12_cryptography__N8_keyStore__S35_GetItemsForInitializeMutationOutput__M13_MutationIndex(concrete._MutationIndex); return converted;
     }
     public static software.amazon.cryptography.keystore.internaldafny.types._IGetItemsForInitializeMutationOutput ToDafny_N3_aws__N12_cryptography__N8_keyStore__S35_GetItemsForInitializeMutationOutput(AWS.Cryptography.KeyStore.GetItemsForInitializeMutationOutput value)
     {
       value.Validate();
       AWS.Cryptography.KeyStore.MutationLock var_mutationLock = value.IsSetMutationLock() ? value.MutationLock : (AWS.Cryptography.KeyStore.MutationLock)null;
-      return new software.amazon.cryptography.keystore.internaldafny.types.GetItemsForInitializeMutationOutput(ToDafny_N3_aws__N12_cryptography__N8_keyStore__S35_GetItemsForInitializeMutationOutput__M10_ActiveItem(value.ActiveItem), ToDafny_N3_aws__N12_cryptography__N8_keyStore__S35_GetItemsForInitializeMutationOutput__M10_BeaconItem(value.BeaconItem), ToDafny_N3_aws__N12_cryptography__N8_keyStore__S35_GetItemsForInitializeMutationOutput__M12_MutationLock(var_mutationLock));
+      AWS.Cryptography.KeyStore.MutationIndex var_mutationIndex = value.IsSetMutationIndex() ? value.MutationIndex : (AWS.Cryptography.KeyStore.MutationIndex)null;
+      return new software.amazon.cryptography.keystore.internaldafny.types.GetItemsForInitializeMutationOutput(ToDafny_N3_aws__N12_cryptography__N8_keyStore__S35_GetItemsForInitializeMutationOutput__M10_ActiveItem(value.ActiveItem), ToDafny_N3_aws__N12_cryptography__N8_keyStore__S35_GetItemsForInitializeMutationOutput__M10_BeaconItem(value.BeaconItem), ToDafny_N3_aws__N12_cryptography__N8_keyStore__S35_GetItemsForInitializeMutationOutput__M12_MutationLock(var_mutationLock), ToDafny_N3_aws__N12_cryptography__N8_keyStore__S35_GetItemsForInitializeMutationOutput__M13_MutationIndex(var_mutationIndex));
     }
     public static AWS.Cryptography.KeyStore.GetKeyStorageInfoInput FromDafny_N3_aws__N12_cryptography__N8_keyStore__S22_GetKeyStorageInfoInput(software.amazon.cryptography.keystore.internaldafny.types._IGetKeyStorageInfoInput value)
     {
@@ -264,6 +266,28 @@ namespace AWS.Cryptography.KeyStore
       value.Validate();
 
       return new software.amazon.cryptography.keystore.internaldafny.types.GetKeyStoreInfoOutput(ToDafny_N3_aws__N12_cryptography__N8_keyStore__S21_GetKeyStoreInfoOutput__M10_keyStoreId(value.KeyStoreId), ToDafny_N3_aws__N12_cryptography__N8_keyStore__S21_GetKeyStoreInfoOutput__M12_keyStoreName(value.KeyStoreName), ToDafny_N3_aws__N12_cryptography__N8_keyStore__S21_GetKeyStoreInfoOutput__M19_logicalKeyStoreName(value.LogicalKeyStoreName), ToDafny_N3_aws__N12_cryptography__N8_keyStore__S21_GetKeyStoreInfoOutput__M11_grantTokens(value.GrantTokens), ToDafny_N3_aws__N12_cryptography__N8_keyStore__S21_GetKeyStoreInfoOutput__M16_kmsConfiguration(value.KmsConfiguration));
+    }
+    public static AWS.Cryptography.KeyStore.GetMutationLockAndIndexInput FromDafny_N3_aws__N12_cryptography__N8_keyStore__S28_GetMutationLockAndIndexInput(software.amazon.cryptography.keystore.internaldafny.types._IGetMutationLockAndIndexInput value)
+    {
+      software.amazon.cryptography.keystore.internaldafny.types.GetMutationLockAndIndexInput concrete = (software.amazon.cryptography.keystore.internaldafny.types.GetMutationLockAndIndexInput)value; AWS.Cryptography.KeyStore.GetMutationLockAndIndexInput converted = new AWS.Cryptography.KeyStore.GetMutationLockAndIndexInput(); converted.Identifier = (string)FromDafny_N3_aws__N12_cryptography__N8_keyStore__S28_GetMutationLockAndIndexInput__M10_Identifier(concrete._Identifier); return converted;
+    }
+    public static software.amazon.cryptography.keystore.internaldafny.types._IGetMutationLockAndIndexInput ToDafny_N3_aws__N12_cryptography__N8_keyStore__S28_GetMutationLockAndIndexInput(AWS.Cryptography.KeyStore.GetMutationLockAndIndexInput value)
+    {
+      value.Validate();
+
+      return new software.amazon.cryptography.keystore.internaldafny.types.GetMutationLockAndIndexInput(ToDafny_N3_aws__N12_cryptography__N8_keyStore__S28_GetMutationLockAndIndexInput__M10_Identifier(value.Identifier));
+    }
+    public static AWS.Cryptography.KeyStore.GetMutationLockAndIndexOutput FromDafny_N3_aws__N12_cryptography__N8_keyStore__S29_GetMutationLockAndIndexOutput(software.amazon.cryptography.keystore.internaldafny.types._IGetMutationLockAndIndexOutput value)
+    {
+      software.amazon.cryptography.keystore.internaldafny.types.GetMutationLockAndIndexOutput concrete = (software.amazon.cryptography.keystore.internaldafny.types.GetMutationLockAndIndexOutput)value; AWS.Cryptography.KeyStore.GetMutationLockAndIndexOutput converted = new AWS.Cryptography.KeyStore.GetMutationLockAndIndexOutput(); if (concrete._MutationLock.is_Some) converted.MutationLock = (AWS.Cryptography.KeyStore.MutationLock)FromDafny_N3_aws__N12_cryptography__N8_keyStore__S29_GetMutationLockAndIndexOutput__M12_MutationLock(concrete._MutationLock);
+      if (concrete._MutationIndex.is_Some) converted.MutationIndex = (AWS.Cryptography.KeyStore.MutationIndex)FromDafny_N3_aws__N12_cryptography__N8_keyStore__S29_GetMutationLockAndIndexOutput__M13_MutationIndex(concrete._MutationIndex); return converted;
+    }
+    public static software.amazon.cryptography.keystore.internaldafny.types._IGetMutationLockAndIndexOutput ToDafny_N3_aws__N12_cryptography__N8_keyStore__S29_GetMutationLockAndIndexOutput(AWS.Cryptography.KeyStore.GetMutationLockAndIndexOutput value)
+    {
+      value.Validate();
+      AWS.Cryptography.KeyStore.MutationLock var_mutationLock = value.IsSetMutationLock() ? value.MutationLock : (AWS.Cryptography.KeyStore.MutationLock)null;
+      AWS.Cryptography.KeyStore.MutationIndex var_mutationIndex = value.IsSetMutationIndex() ? value.MutationIndex : (AWS.Cryptography.KeyStore.MutationIndex)null;
+      return new software.amazon.cryptography.keystore.internaldafny.types.GetMutationLockAndIndexOutput(ToDafny_N3_aws__N12_cryptography__N8_keyStore__S29_GetMutationLockAndIndexOutput__M12_MutationLock(var_mutationLock), ToDafny_N3_aws__N12_cryptography__N8_keyStore__S29_GetMutationLockAndIndexOutput__M13_MutationIndex(var_mutationIndex));
     }
     public static AWS.Cryptography.KeyStore.GetMutationLockInput FromDafny_N3_aws__N12_cryptography__N8_keyStore__S20_GetMutationLockInput(software.amazon.cryptography.keystore.internaldafny.types._IGetMutationLockInput value)
     {
@@ -488,26 +512,26 @@ namespace AWS.Cryptography.KeyStore
     }
     public static AWS.Cryptography.KeyStore.QueryForVersionsInput FromDafny_N3_aws__N12_cryptography__N8_keyStore__S21_QueryForVersionsInput(software.amazon.cryptography.keystore.internaldafny.types._IQueryForVersionsInput value)
     {
-      software.amazon.cryptography.keystore.internaldafny.types.QueryForVersionsInput concrete = (software.amazon.cryptography.keystore.internaldafny.types.QueryForVersionsInput)value; AWS.Cryptography.KeyStore.QueryForVersionsInput converted = new AWS.Cryptography.KeyStore.QueryForVersionsInput(); if (concrete._ExclusiveStartKey.is_Some) converted.ExclusiveStartKey = (System.IO.MemoryStream)FromDafny_N3_aws__N12_cryptography__N8_keyStore__S21_QueryForVersionsInput__M17_ExclusiveStartKey(concrete._ExclusiveStartKey);
+      software.amazon.cryptography.keystore.internaldafny.types.QueryForVersionsInput concrete = (software.amazon.cryptography.keystore.internaldafny.types.QueryForVersionsInput)value; AWS.Cryptography.KeyStore.QueryForVersionsInput converted = new AWS.Cryptography.KeyStore.QueryForVersionsInput(); if (concrete._PageIndex.is_Some) converted.PageIndex = (System.IO.MemoryStream)FromDafny_N3_aws__N12_cryptography__N8_keyStore__S21_QueryForVersionsInput__M9_PageIndex(concrete._PageIndex);
       converted.Identifier = (string)FromDafny_N3_aws__N12_cryptography__N8_keyStore__S21_QueryForVersionsInput__M10_Identifier(concrete._Identifier);
       converted.PageSize = (int)FromDafny_N3_aws__N12_cryptography__N8_keyStore__S21_QueryForVersionsInput__M8_PageSize(concrete._PageSize); return converted;
     }
     public static software.amazon.cryptography.keystore.internaldafny.types._IQueryForVersionsInput ToDafny_N3_aws__N12_cryptography__N8_keyStore__S21_QueryForVersionsInput(AWS.Cryptography.KeyStore.QueryForVersionsInput value)
     {
       value.Validate();
-      System.IO.MemoryStream var_exclusiveStartKey = value.IsSetExclusiveStartKey() ? value.ExclusiveStartKey : (System.IO.MemoryStream)null;
-      return new software.amazon.cryptography.keystore.internaldafny.types.QueryForVersionsInput(ToDafny_N3_aws__N12_cryptography__N8_keyStore__S21_QueryForVersionsInput__M17_ExclusiveStartKey(var_exclusiveStartKey), ToDafny_N3_aws__N12_cryptography__N8_keyStore__S21_QueryForVersionsInput__M10_Identifier(value.Identifier), ToDafny_N3_aws__N12_cryptography__N8_keyStore__S21_QueryForVersionsInput__M8_PageSize(value.PageSize));
+      System.IO.MemoryStream var_pageIndex = value.IsSetPageIndex() ? value.PageIndex : (System.IO.MemoryStream)null;
+      return new software.amazon.cryptography.keystore.internaldafny.types.QueryForVersionsInput(ToDafny_N3_aws__N12_cryptography__N8_keyStore__S21_QueryForVersionsInput__M9_PageIndex(var_pageIndex), ToDafny_N3_aws__N12_cryptography__N8_keyStore__S21_QueryForVersionsInput__M10_Identifier(value.Identifier), ToDafny_N3_aws__N12_cryptography__N8_keyStore__S21_QueryForVersionsInput__M8_PageSize(value.PageSize));
     }
     public static AWS.Cryptography.KeyStore.QueryForVersionsOutput FromDafny_N3_aws__N12_cryptography__N8_keyStore__S22_QueryForVersionsOutput(software.amazon.cryptography.keystore.internaldafny.types._IQueryForVersionsOutput value)
     {
-      software.amazon.cryptography.keystore.internaldafny.types.QueryForVersionsOutput concrete = (software.amazon.cryptography.keystore.internaldafny.types.QueryForVersionsOutput)value; AWS.Cryptography.KeyStore.QueryForVersionsOutput converted = new AWS.Cryptography.KeyStore.QueryForVersionsOutput(); converted.ExclusiveStartKey = (System.IO.MemoryStream)FromDafny_N3_aws__N12_cryptography__N8_keyStore__S22_QueryForVersionsOutput__M17_ExclusiveStartKey(concrete._ExclusiveStartKey);
+      software.amazon.cryptography.keystore.internaldafny.types.QueryForVersionsOutput concrete = (software.amazon.cryptography.keystore.internaldafny.types.QueryForVersionsOutput)value; AWS.Cryptography.KeyStore.QueryForVersionsOutput converted = new AWS.Cryptography.KeyStore.QueryForVersionsOutput(); converted.PageIndex = (System.IO.MemoryStream)FromDafny_N3_aws__N12_cryptography__N8_keyStore__S22_QueryForVersionsOutput__M9_PageIndex(concrete._PageIndex);
       converted.Items = (System.Collections.Generic.List<AWS.Cryptography.KeyStore.EncryptedHierarchicalKey>)FromDafny_N3_aws__N12_cryptography__N8_keyStore__S22_QueryForVersionsOutput__M5_Items(concrete._Items); return converted;
     }
     public static software.amazon.cryptography.keystore.internaldafny.types._IQueryForVersionsOutput ToDafny_N3_aws__N12_cryptography__N8_keyStore__S22_QueryForVersionsOutput(AWS.Cryptography.KeyStore.QueryForVersionsOutput value)
     {
       value.Validate();
 
-      return new software.amazon.cryptography.keystore.internaldafny.types.QueryForVersionsOutput(ToDafny_N3_aws__N12_cryptography__N8_keyStore__S22_QueryForVersionsOutput__M17_ExclusiveStartKey(value.ExclusiveStartKey), ToDafny_N3_aws__N12_cryptography__N8_keyStore__S22_QueryForVersionsOutput__M5_Items(value.Items));
+      return new software.amazon.cryptography.keystore.internaldafny.types.QueryForVersionsOutput(ToDafny_N3_aws__N12_cryptography__N8_keyStore__S22_QueryForVersionsOutput__M9_PageIndex(value.PageIndex), ToDafny_N3_aws__N12_cryptography__N8_keyStore__S22_QueryForVersionsOutput__M5_Items(value.Items));
     }
     public static AWS.Cryptography.KeyStore.Storage FromDafny_N3_aws__N12_cryptography__N8_keyStore__S7_Storage(software.amazon.cryptography.keystore.internaldafny.types._IStorage value)
     {
@@ -535,6 +559,27 @@ namespace AWS.Cryptography.KeyStore
         return software.amazon.cryptography.keystore.internaldafny.types.Storage.create_custom(ToDafny_N3_aws__N12_cryptography__N8_keyStore__S7_Storage__M6_custom(value.Custom));
       }
       throw new System.ArgumentException("Invalid AWS.Cryptography.KeyStore.Storage state");
+    }
+    public static AWS.Cryptography.KeyStore.UpdateMutationIndexInput FromDafny_N3_aws__N12_cryptography__N8_keyStore__S24_UpdateMutationIndexInput(software.amazon.cryptography.keystore.internaldafny.types._IUpdateMutationIndexInput value)
+    {
+      software.amazon.cryptography.keystore.internaldafny.types.UpdateMutationIndexInput concrete = (software.amazon.cryptography.keystore.internaldafny.types.UpdateMutationIndexInput)value; AWS.Cryptography.KeyStore.UpdateMutationIndexInput converted = new AWS.Cryptography.KeyStore.UpdateMutationIndexInput(); converted.MutationIndex = (AWS.Cryptography.KeyStore.MutationIndex)FromDafny_N3_aws__N12_cryptography__N8_keyStore__S24_UpdateMutationIndexInput__M13_MutationIndex(concrete._MutationIndex);
+      converted.OldMutationIndex = (AWS.Cryptography.KeyStore.MutationIndex)FromDafny_N3_aws__N12_cryptography__N8_keyStore__S24_UpdateMutationIndexInput__M16_OldMutationIndex(concrete._OldMutationIndex); return converted;
+    }
+    public static software.amazon.cryptography.keystore.internaldafny.types._IUpdateMutationIndexInput ToDafny_N3_aws__N12_cryptography__N8_keyStore__S24_UpdateMutationIndexInput(AWS.Cryptography.KeyStore.UpdateMutationIndexInput value)
+    {
+      value.Validate();
+
+      return new software.amazon.cryptography.keystore.internaldafny.types.UpdateMutationIndexInput(ToDafny_N3_aws__N12_cryptography__N8_keyStore__S24_UpdateMutationIndexInput__M13_MutationIndex(value.MutationIndex), ToDafny_N3_aws__N12_cryptography__N8_keyStore__S24_UpdateMutationIndexInput__M16_OldMutationIndex(value.OldMutationIndex));
+    }
+    public static AWS.Cryptography.KeyStore.UpdateMutationIndexOutput FromDafny_N3_aws__N12_cryptography__N8_keyStore__S25_UpdateMutationIndexOutput(software.amazon.cryptography.keystore.internaldafny.types._IUpdateMutationIndexOutput value)
+    {
+      software.amazon.cryptography.keystore.internaldafny.types.UpdateMutationIndexOutput concrete = (software.amazon.cryptography.keystore.internaldafny.types.UpdateMutationIndexOutput)value; AWS.Cryptography.KeyStore.UpdateMutationIndexOutput converted = new AWS.Cryptography.KeyStore.UpdateMutationIndexOutput(); return converted;
+    }
+    public static software.amazon.cryptography.keystore.internaldafny.types._IUpdateMutationIndexOutput ToDafny_N3_aws__N12_cryptography__N8_keyStore__S25_UpdateMutationIndexOutput(AWS.Cryptography.KeyStore.UpdateMutationIndexOutput value)
+    {
+      value.Validate();
+
+      return new software.amazon.cryptography.keystore.internaldafny.types.UpdateMutationIndexOutput();
     }
     public static AWS.Cryptography.KeyStore.VersionKeyInput FromDafny_N3_aws__N12_cryptography__N8_keyStore__S15_VersionKeyInput(software.amazon.cryptography.keystore.internaldafny.types._IVersionKeyInput value)
     {
@@ -571,17 +616,17 @@ namespace AWS.Cryptography.KeyStore
     }
     public static AWS.Cryptography.KeyStore.WriteInitializeMutationInput FromDafny_N3_aws__N12_cryptography__N8_keyStore__S28_WriteInitializeMutationInput(software.amazon.cryptography.keystore.internaldafny.types._IWriteInitializeMutationInput value)
     {
-      software.amazon.cryptography.keystore.internaldafny.types.WriteInitializeMutationInput concrete = (software.amazon.cryptography.keystore.internaldafny.types.WriteInitializeMutationInput)value; AWS.Cryptography.KeyStore.WriteInitializeMutationInput converted = new AWS.Cryptography.KeyStore.WriteInitializeMutationInput(); converted.Active = (AWS.Cryptography.KeyStore.EncryptedHierarchicalKey)FromDafny_N3_aws__N12_cryptography__N8_keyStore__S28_WriteInitializeMutationInput__M6_Active(concrete._Active);
-      converted.OldActive = (AWS.Cryptography.KeyStore.EncryptedHierarchicalKey)FromDafny_N3_aws__N12_cryptography__N8_keyStore__S28_WriteInitializeMutationInput__M9_OldActive(concrete._OldActive);
+      software.amazon.cryptography.keystore.internaldafny.types.WriteInitializeMutationInput concrete = (software.amazon.cryptography.keystore.internaldafny.types.WriteInitializeMutationInput)value; AWS.Cryptography.KeyStore.WriteInitializeMutationInput converted = new AWS.Cryptography.KeyStore.WriteInitializeMutationInput(); converted.Active = (AWS.Cryptography.KeyStore.OverWriteEncryptedHierarchicalKey)FromDafny_N3_aws__N12_cryptography__N8_keyStore__S28_WriteInitializeMutationInput__M6_Active(concrete._Active);
       converted.Version = (AWS.Cryptography.KeyStore.EncryptedHierarchicalKey)FromDafny_N3_aws__N12_cryptography__N8_keyStore__S28_WriteInitializeMutationInput__M7_Version(concrete._Version);
-      converted.Beacon = (AWS.Cryptography.KeyStore.EncryptedHierarchicalKey)FromDafny_N3_aws__N12_cryptography__N8_keyStore__S28_WriteInitializeMutationInput__M6_Beacon(concrete._Beacon);
-      converted.MutationLock = (AWS.Cryptography.KeyStore.MutationLock)FromDafny_N3_aws__N12_cryptography__N8_keyStore__S28_WriteInitializeMutationInput__M12_MutationLock(concrete._MutationLock); return converted;
+      converted.Beacon = (AWS.Cryptography.KeyStore.OverWriteEncryptedHierarchicalKey)FromDafny_N3_aws__N12_cryptography__N8_keyStore__S28_WriteInitializeMutationInput__M6_Beacon(concrete._Beacon);
+      converted.MutationLock = (AWS.Cryptography.KeyStore.MutationLock)FromDafny_N3_aws__N12_cryptography__N8_keyStore__S28_WriteInitializeMutationInput__M12_MutationLock(concrete._MutationLock);
+      converted.MutationIndex = (AWS.Cryptography.KeyStore.MutationIndex)FromDafny_N3_aws__N12_cryptography__N8_keyStore__S28_WriteInitializeMutationInput__M13_MutationIndex(concrete._MutationIndex); return converted;
     }
     public static software.amazon.cryptography.keystore.internaldafny.types._IWriteInitializeMutationInput ToDafny_N3_aws__N12_cryptography__N8_keyStore__S28_WriteInitializeMutationInput(AWS.Cryptography.KeyStore.WriteInitializeMutationInput value)
     {
       value.Validate();
 
-      return new software.amazon.cryptography.keystore.internaldafny.types.WriteInitializeMutationInput(ToDafny_N3_aws__N12_cryptography__N8_keyStore__S28_WriteInitializeMutationInput__M6_Active(value.Active), ToDafny_N3_aws__N12_cryptography__N8_keyStore__S28_WriteInitializeMutationInput__M9_OldActive(value.OldActive), ToDafny_N3_aws__N12_cryptography__N8_keyStore__S28_WriteInitializeMutationInput__M7_Version(value.Version), ToDafny_N3_aws__N12_cryptography__N8_keyStore__S28_WriteInitializeMutationInput__M6_Beacon(value.Beacon), ToDafny_N3_aws__N12_cryptography__N8_keyStore__S28_WriteInitializeMutationInput__M12_MutationLock(value.MutationLock));
+      return new software.amazon.cryptography.keystore.internaldafny.types.WriteInitializeMutationInput(ToDafny_N3_aws__N12_cryptography__N8_keyStore__S28_WriteInitializeMutationInput__M6_Active(value.Active), ToDafny_N3_aws__N12_cryptography__N8_keyStore__S28_WriteInitializeMutationInput__M7_Version(value.Version), ToDafny_N3_aws__N12_cryptography__N8_keyStore__S28_WriteInitializeMutationInput__M6_Beacon(value.Beacon), ToDafny_N3_aws__N12_cryptography__N8_keyStore__S28_WriteInitializeMutationInput__M12_MutationLock(value.MutationLock), ToDafny_N3_aws__N12_cryptography__N8_keyStore__S28_WriteInitializeMutationInput__M13_MutationIndex(value.MutationIndex));
     }
     public static AWS.Cryptography.KeyStore.WriteInitializeMutationOutput FromDafny_N3_aws__N12_cryptography__N8_keyStore__S29_WriteInitializeMutationOutput(software.amazon.cryptography.keystore.internaldafny.types._IWriteInitializeMutationOutput value)
     {
@@ -595,17 +640,14 @@ namespace AWS.Cryptography.KeyStore
     }
     public static AWS.Cryptography.KeyStore.WriteMutatedVersionsInput FromDafny_N3_aws__N12_cryptography__N8_keyStore__S25_WriteMutatedVersionsInput(software.amazon.cryptography.keystore.internaldafny.types._IWriteMutatedVersionsInput value)
     {
-      software.amazon.cryptography.keystore.internaldafny.types.WriteMutatedVersionsInput concrete = (software.amazon.cryptography.keystore.internaldafny.types.WriteMutatedVersionsInput)value; AWS.Cryptography.KeyStore.WriteMutatedVersionsInput converted = new AWS.Cryptography.KeyStore.WriteMutatedVersionsInput(); converted.Items = (System.Collections.Generic.List<AWS.Cryptography.KeyStore.EncryptedHierarchicalKey>)FromDafny_N3_aws__N12_cryptography__N8_keyStore__S25_WriteMutatedVersionsInput__M5_Items(concrete._Items);
-      converted.Identifier = (string)FromDafny_N3_aws__N12_cryptography__N8_keyStore__S25_WriteMutatedVersionsInput__M10_Identifier(concrete._Identifier);
-      converted.Original = (System.IO.MemoryStream)FromDafny_N3_aws__N12_cryptography__N8_keyStore__S25_WriteMutatedVersionsInput__M8_Original(concrete._Original);
-      converted.Terminal = (System.IO.MemoryStream)FromDafny_N3_aws__N12_cryptography__N8_keyStore__S25_WriteMutatedVersionsInput__M8_Terminal(concrete._Terminal);
-      converted.CompleteMutation = (bool)FromDafny_N3_aws__N12_cryptography__N8_keyStore__S25_WriteMutatedVersionsInput__M16_CompleteMutation(concrete._CompleteMutation); return converted;
+      software.amazon.cryptography.keystore.internaldafny.types.WriteMutatedVersionsInput concrete = (software.amazon.cryptography.keystore.internaldafny.types.WriteMutatedVersionsInput)value; AWS.Cryptography.KeyStore.WriteMutatedVersionsInput converted = new AWS.Cryptography.KeyStore.WriteMutatedVersionsInput(); converted.Items = (System.Collections.Generic.List<AWS.Cryptography.KeyStore.OverWriteEncryptedHierarchicalKey>)FromDafny_N3_aws__N12_cryptography__N8_keyStore__S25_WriteMutatedVersionsInput__M5_Items(concrete._Items);
+      converted.MutationLock = (AWS.Cryptography.KeyStore.MutationLock)FromDafny_N3_aws__N12_cryptography__N8_keyStore__S25_WriteMutatedVersionsInput__M12_MutationLock(concrete._MutationLock); return converted;
     }
     public static software.amazon.cryptography.keystore.internaldafny.types._IWriteMutatedVersionsInput ToDafny_N3_aws__N12_cryptography__N8_keyStore__S25_WriteMutatedVersionsInput(AWS.Cryptography.KeyStore.WriteMutatedVersionsInput value)
     {
       value.Validate();
 
-      return new software.amazon.cryptography.keystore.internaldafny.types.WriteMutatedVersionsInput(ToDafny_N3_aws__N12_cryptography__N8_keyStore__S25_WriteMutatedVersionsInput__M5_Items(value.Items), ToDafny_N3_aws__N12_cryptography__N8_keyStore__S25_WriteMutatedVersionsInput__M10_Identifier(value.Identifier), ToDafny_N3_aws__N12_cryptography__N8_keyStore__S25_WriteMutatedVersionsInput__M8_Original(value.Original), ToDafny_N3_aws__N12_cryptography__N8_keyStore__S25_WriteMutatedVersionsInput__M8_Terminal(value.Terminal), ToDafny_N3_aws__N12_cryptography__N8_keyStore__S25_WriteMutatedVersionsInput__M16_CompleteMutation(value.CompleteMutation));
+      return new software.amazon.cryptography.keystore.internaldafny.types.WriteMutatedVersionsInput(ToDafny_N3_aws__N12_cryptography__N8_keyStore__S25_WriteMutatedVersionsInput__M5_Items(value.Items), ToDafny_N3_aws__N12_cryptography__N8_keyStore__S25_WriteMutatedVersionsInput__M12_MutationLock(value.MutationLock));
     }
     public static AWS.Cryptography.KeyStore.WriteMutatedVersionsOutput FromDafny_N3_aws__N12_cryptography__N8_keyStore__S26_WriteMutatedVersionsOutput(software.amazon.cryptography.keystore.internaldafny.types._IWriteMutatedVersionsOutput value)
     {
@@ -641,15 +683,14 @@ namespace AWS.Cryptography.KeyStore
     }
     public static AWS.Cryptography.KeyStore.WriteNewEncryptedBranchKeyVersionInput FromDafny_N3_aws__N12_cryptography__N8_keyStore__S38_WriteNewEncryptedBranchKeyVersionInput(software.amazon.cryptography.keystore.internaldafny.types._IWriteNewEncryptedBranchKeyVersionInput value)
     {
-      software.amazon.cryptography.keystore.internaldafny.types.WriteNewEncryptedBranchKeyVersionInput concrete = (software.amazon.cryptography.keystore.internaldafny.types.WriteNewEncryptedBranchKeyVersionInput)value; AWS.Cryptography.KeyStore.WriteNewEncryptedBranchKeyVersionInput converted = new AWS.Cryptography.KeyStore.WriteNewEncryptedBranchKeyVersionInput(); converted.Active = (AWS.Cryptography.KeyStore.EncryptedHierarchicalKey)FromDafny_N3_aws__N12_cryptography__N8_keyStore__S38_WriteNewEncryptedBranchKeyVersionInput__M6_Active(concrete._Active);
-      converted.Version = (AWS.Cryptography.KeyStore.EncryptedHierarchicalKey)FromDafny_N3_aws__N12_cryptography__N8_keyStore__S38_WriteNewEncryptedBranchKeyVersionInput__M7_Version(concrete._Version);
-      converted.OldActive = (AWS.Cryptography.KeyStore.EncryptedHierarchicalKey)FromDafny_N3_aws__N12_cryptography__N8_keyStore__S38_WriteNewEncryptedBranchKeyVersionInput__M9_OldActive(concrete._OldActive); return converted;
+      software.amazon.cryptography.keystore.internaldafny.types.WriteNewEncryptedBranchKeyVersionInput concrete = (software.amazon.cryptography.keystore.internaldafny.types.WriteNewEncryptedBranchKeyVersionInput)value; AWS.Cryptography.KeyStore.WriteNewEncryptedBranchKeyVersionInput converted = new AWS.Cryptography.KeyStore.WriteNewEncryptedBranchKeyVersionInput(); converted.Active = (AWS.Cryptography.KeyStore.OverWriteEncryptedHierarchicalKey)FromDafny_N3_aws__N12_cryptography__N8_keyStore__S38_WriteNewEncryptedBranchKeyVersionInput__M6_Active(concrete._Active);
+      converted.Version = (AWS.Cryptography.KeyStore.EncryptedHierarchicalKey)FromDafny_N3_aws__N12_cryptography__N8_keyStore__S38_WriteNewEncryptedBranchKeyVersionInput__M7_Version(concrete._Version); return converted;
     }
     public static software.amazon.cryptography.keystore.internaldafny.types._IWriteNewEncryptedBranchKeyVersionInput ToDafny_N3_aws__N12_cryptography__N8_keyStore__S38_WriteNewEncryptedBranchKeyVersionInput(AWS.Cryptography.KeyStore.WriteNewEncryptedBranchKeyVersionInput value)
     {
       value.Validate();
 
-      return new software.amazon.cryptography.keystore.internaldafny.types.WriteNewEncryptedBranchKeyVersionInput(ToDafny_N3_aws__N12_cryptography__N8_keyStore__S38_WriteNewEncryptedBranchKeyVersionInput__M6_Active(value.Active), ToDafny_N3_aws__N12_cryptography__N8_keyStore__S38_WriteNewEncryptedBranchKeyVersionInput__M7_Version(value.Version), ToDafny_N3_aws__N12_cryptography__N8_keyStore__S38_WriteNewEncryptedBranchKeyVersionInput__M9_OldActive(value.OldActive));
+      return new software.amazon.cryptography.keystore.internaldafny.types.WriteNewEncryptedBranchKeyVersionInput(ToDafny_N3_aws__N12_cryptography__N8_keyStore__S38_WriteNewEncryptedBranchKeyVersionInput__M6_Active(value.Active), ToDafny_N3_aws__N12_cryptography__N8_keyStore__S38_WriteNewEncryptedBranchKeyVersionInput__M7_Version(value.Version));
     }
     public static AWS.Cryptography.KeyStore.WriteNewEncryptedBranchKeyVersionOutput FromDafny_N3_aws__N12_cryptography__N8_keyStore__S39_WriteNewEncryptedBranchKeyVersionOutput(software.amazon.cryptography.keystore.internaldafny.types._IWriteNewEncryptedBranchKeyVersionOutput value)
     {
@@ -668,14 +709,6 @@ namespace AWS.Cryptography.KeyStore
     public static Dafny.ISequence<char> ToDafny_N3_aws__N12_cryptography__N8_keyStore__S28_AlreadyExistsConditionFailed__M7_message(string value)
     {
       return ToDafny_N6_smithy__N3_api__S6_String(value);
-    }
-    public static AWS.Cryptography.KeyStore.MutationLock FromDafny_N3_aws__N12_cryptography__N8_keyStore__S24_ClobberMutationLockInput__M12_MutationLock(software.amazon.cryptography.keystore.internaldafny.types._IMutationLock value)
-    {
-      return FromDafny_N3_aws__N12_cryptography__N8_keyStore__S12_MutationLock(value);
-    }
-    public static software.amazon.cryptography.keystore.internaldafny.types._IMutationLock ToDafny_N3_aws__N12_cryptography__N8_keyStore__S24_ClobberMutationLockInput__M12_MutationLock(AWS.Cryptography.KeyStore.MutationLock value)
-    {
-      return ToDafny_N3_aws__N12_cryptography__N8_keyStore__S12_MutationLock(value);
     }
     public static string FromDafny_N3_aws__N12_cryptography__N8_keyStore__S14_CreateKeyInput__M19_branchKeyIdentifier(Wrappers_Compile._IOption<Dafny.ISequence<char>> value)
     {
@@ -708,6 +741,14 @@ namespace AWS.Cryptography.KeyStore
     public static Dafny.ISequence<char> ToDafny_N3_aws__N12_cryptography__N8_keyStore__S20_CreateKeyStoreOutput__M8_tableArn(string value)
     {
       return ToDafny_N3_com__N9_amazonaws__N8_dynamodb__S8_TableArn(value);
+    }
+    public static AWS.Cryptography.KeyStore.MutationLock FromDafny_N3_aws__N12_cryptography__N8_keyStore__S31_DeleteMutationLockAndIndexInput__M12_MutationLock(software.amazon.cryptography.keystore.internaldafny.types._IMutationLock value)
+    {
+      return FromDafny_N3_aws__N12_cryptography__N8_keyStore__S12_MutationLock(value);
+    }
+    public static software.amazon.cryptography.keystore.internaldafny.types._IMutationLock ToDafny_N3_aws__N12_cryptography__N8_keyStore__S31_DeleteMutationLockAndIndexInput__M12_MutationLock(AWS.Cryptography.KeyStore.MutationLock value)
+    {
+      return ToDafny_N3_aws__N12_cryptography__N8_keyStore__S12_MutationLock(value);
     }
     public static string FromDafny_N3_aws__N12_cryptography__N8_keyStore__S23_GetActiveBranchKeyInput__M19_branchKeyIdentifier(Dafny.ISequence<char> value)
     {
@@ -853,6 +894,14 @@ namespace AWS.Cryptography.KeyStore
     {
       return value == null ? Wrappers_Compile.Option<software.amazon.cryptography.keystore.internaldafny.types._IMutationLock>.create_None() : Wrappers_Compile.Option<software.amazon.cryptography.keystore.internaldafny.types._IMutationLock>.create_Some(ToDafny_N3_aws__N12_cryptography__N8_keyStore__S12_MutationLock((AWS.Cryptography.KeyStore.MutationLock)value));
     }
+    public static AWS.Cryptography.KeyStore.MutationIndex FromDafny_N3_aws__N12_cryptography__N8_keyStore__S35_GetItemsForInitializeMutationOutput__M13_MutationIndex(Wrappers_Compile._IOption<software.amazon.cryptography.keystore.internaldafny.types._IMutationIndex> value)
+    {
+      return value.is_None ? (AWS.Cryptography.KeyStore.MutationIndex)null : FromDafny_N3_aws__N12_cryptography__N8_keyStore__S13_MutationIndex(value.Extract());
+    }
+    public static Wrappers_Compile._IOption<software.amazon.cryptography.keystore.internaldafny.types._IMutationIndex> ToDafny_N3_aws__N12_cryptography__N8_keyStore__S35_GetItemsForInitializeMutationOutput__M13_MutationIndex(AWS.Cryptography.KeyStore.MutationIndex value)
+    {
+      return value == null ? Wrappers_Compile.Option<software.amazon.cryptography.keystore.internaldafny.types._IMutationIndex>.create_None() : Wrappers_Compile.Option<software.amazon.cryptography.keystore.internaldafny.types._IMutationIndex>.create_Some(ToDafny_N3_aws__N12_cryptography__N8_keyStore__S13_MutationIndex((AWS.Cryptography.KeyStore.MutationIndex)value));
+    }
     public static string FromDafny_N3_aws__N12_cryptography__N8_keyStore__S23_GetKeyStorageInfoOutput__M4_Name(Dafny.ISequence<byte> value)
     {
       return FromDafny_N3_aws__N12_cryptography__N8_keyStore__S9_Utf8Bytes(value);
@@ -908,6 +957,30 @@ namespace AWS.Cryptography.KeyStore
     public static software.amazon.cryptography.keystore.internaldafny.types._IKMSConfiguration ToDafny_N3_aws__N12_cryptography__N8_keyStore__S21_GetKeyStoreInfoOutput__M16_kmsConfiguration(AWS.Cryptography.KeyStore.KMSConfiguration value)
     {
       return ToDafny_N3_aws__N12_cryptography__N8_keyStore__S16_KMSConfiguration(value);
+    }
+    public static string FromDafny_N3_aws__N12_cryptography__N8_keyStore__S28_GetMutationLockAndIndexInput__M10_Identifier(Dafny.ISequence<char> value)
+    {
+      return FromDafny_N6_smithy__N3_api__S6_String(value);
+    }
+    public static Dafny.ISequence<char> ToDafny_N3_aws__N12_cryptography__N8_keyStore__S28_GetMutationLockAndIndexInput__M10_Identifier(string value)
+    {
+      return ToDafny_N6_smithy__N3_api__S6_String(value);
+    }
+    public static AWS.Cryptography.KeyStore.MutationLock FromDafny_N3_aws__N12_cryptography__N8_keyStore__S29_GetMutationLockAndIndexOutput__M12_MutationLock(Wrappers_Compile._IOption<software.amazon.cryptography.keystore.internaldafny.types._IMutationLock> value)
+    {
+      return value.is_None ? (AWS.Cryptography.KeyStore.MutationLock)null : FromDafny_N3_aws__N12_cryptography__N8_keyStore__S12_MutationLock(value.Extract());
+    }
+    public static Wrappers_Compile._IOption<software.amazon.cryptography.keystore.internaldafny.types._IMutationLock> ToDafny_N3_aws__N12_cryptography__N8_keyStore__S29_GetMutationLockAndIndexOutput__M12_MutationLock(AWS.Cryptography.KeyStore.MutationLock value)
+    {
+      return value == null ? Wrappers_Compile.Option<software.amazon.cryptography.keystore.internaldafny.types._IMutationLock>.create_None() : Wrappers_Compile.Option<software.amazon.cryptography.keystore.internaldafny.types._IMutationLock>.create_Some(ToDafny_N3_aws__N12_cryptography__N8_keyStore__S12_MutationLock((AWS.Cryptography.KeyStore.MutationLock)value));
+    }
+    public static AWS.Cryptography.KeyStore.MutationIndex FromDafny_N3_aws__N12_cryptography__N8_keyStore__S29_GetMutationLockAndIndexOutput__M13_MutationIndex(Wrappers_Compile._IOption<software.amazon.cryptography.keystore.internaldafny.types._IMutationIndex> value)
+    {
+      return value.is_None ? (AWS.Cryptography.KeyStore.MutationIndex)null : FromDafny_N3_aws__N12_cryptography__N8_keyStore__S13_MutationIndex(value.Extract());
+    }
+    public static Wrappers_Compile._IOption<software.amazon.cryptography.keystore.internaldafny.types._IMutationIndex> ToDafny_N3_aws__N12_cryptography__N8_keyStore__S29_GetMutationLockAndIndexOutput__M13_MutationIndex(AWS.Cryptography.KeyStore.MutationIndex value)
+    {
+      return value == null ? Wrappers_Compile.Option<software.amazon.cryptography.keystore.internaldafny.types._IMutationIndex>.create_None() : Wrappers_Compile.Option<software.amazon.cryptography.keystore.internaldafny.types._IMutationIndex>.create_Some(ToDafny_N3_aws__N12_cryptography__N8_keyStore__S13_MutationIndex((AWS.Cryptography.KeyStore.MutationIndex)value));
     }
     public static string FromDafny_N3_aws__N12_cryptography__N8_keyStore__S20_GetMutationLockInput__M10_Identifier(Dafny.ISequence<char> value)
     {
@@ -1109,11 +1182,11 @@ namespace AWS.Cryptography.KeyStore
     {
       return ToDafny_N6_smithy__N3_api__S6_String(value);
     }
-    public static System.IO.MemoryStream FromDafny_N3_aws__N12_cryptography__N8_keyStore__S21_QueryForVersionsInput__M17_ExclusiveStartKey(Wrappers_Compile._IOption<Dafny.ISequence<byte>> value)
+    public static System.IO.MemoryStream FromDafny_N3_aws__N12_cryptography__N8_keyStore__S21_QueryForVersionsInput__M9_PageIndex(Wrappers_Compile._IOption<Dafny.ISequence<byte>> value)
     {
       return value.is_None ? (System.IO.MemoryStream)null : FromDafny_N6_smithy__N3_api__S4_Blob(value.Extract());
     }
-    public static Wrappers_Compile._IOption<Dafny.ISequence<byte>> ToDafny_N3_aws__N12_cryptography__N8_keyStore__S21_QueryForVersionsInput__M17_ExclusiveStartKey(System.IO.MemoryStream value)
+    public static Wrappers_Compile._IOption<Dafny.ISequence<byte>> ToDafny_N3_aws__N12_cryptography__N8_keyStore__S21_QueryForVersionsInput__M9_PageIndex(System.IO.MemoryStream value)
     {
       return value == null ? Wrappers_Compile.Option<Dafny.ISequence<byte>>.create_None() : Wrappers_Compile.Option<Dafny.ISequence<byte>>.create_Some(ToDafny_N6_smithy__N3_api__S4_Blob((System.IO.MemoryStream)value));
     }
@@ -1133,11 +1206,11 @@ namespace AWS.Cryptography.KeyStore
     {
       return ToDafny_N6_smithy__N3_api__S7_Integer(value);
     }
-    public static System.IO.MemoryStream FromDafny_N3_aws__N12_cryptography__N8_keyStore__S22_QueryForVersionsOutput__M17_ExclusiveStartKey(Dafny.ISequence<byte> value)
+    public static System.IO.MemoryStream FromDafny_N3_aws__N12_cryptography__N8_keyStore__S22_QueryForVersionsOutput__M9_PageIndex(Dafny.ISequence<byte> value)
     {
       return FromDafny_N6_smithy__N3_api__S4_Blob(value);
     }
-    public static Dafny.ISequence<byte> ToDafny_N3_aws__N12_cryptography__N8_keyStore__S22_QueryForVersionsOutput__M17_ExclusiveStartKey(System.IO.MemoryStream value)
+    public static Dafny.ISequence<byte> ToDafny_N3_aws__N12_cryptography__N8_keyStore__S22_QueryForVersionsOutput__M9_PageIndex(System.IO.MemoryStream value)
     {
       return ToDafny_N6_smithy__N3_api__S4_Blob(value);
     }
@@ -1165,6 +1238,22 @@ namespace AWS.Cryptography.KeyStore
     {
       return ToDafny_N3_aws__N12_cryptography__N8_keyStore__S28_KeyStorageInterfaceReference(value);
     }
+    public static AWS.Cryptography.KeyStore.MutationIndex FromDafny_N3_aws__N12_cryptography__N8_keyStore__S24_UpdateMutationIndexInput__M13_MutationIndex(software.amazon.cryptography.keystore.internaldafny.types._IMutationIndex value)
+    {
+      return FromDafny_N3_aws__N12_cryptography__N8_keyStore__S13_MutationIndex(value);
+    }
+    public static software.amazon.cryptography.keystore.internaldafny.types._IMutationIndex ToDafny_N3_aws__N12_cryptography__N8_keyStore__S24_UpdateMutationIndexInput__M13_MutationIndex(AWS.Cryptography.KeyStore.MutationIndex value)
+    {
+      return ToDafny_N3_aws__N12_cryptography__N8_keyStore__S13_MutationIndex(value);
+    }
+    public static AWS.Cryptography.KeyStore.MutationIndex FromDafny_N3_aws__N12_cryptography__N8_keyStore__S24_UpdateMutationIndexInput__M16_OldMutationIndex(software.amazon.cryptography.keystore.internaldafny.types._IMutationIndex value)
+    {
+      return FromDafny_N3_aws__N12_cryptography__N8_keyStore__S13_MutationIndex(value);
+    }
+    public static software.amazon.cryptography.keystore.internaldafny.types._IMutationIndex ToDafny_N3_aws__N12_cryptography__N8_keyStore__S24_UpdateMutationIndexInput__M16_OldMutationIndex(AWS.Cryptography.KeyStore.MutationIndex value)
+    {
+      return ToDafny_N3_aws__N12_cryptography__N8_keyStore__S13_MutationIndex(value);
+    }
     public static string FromDafny_N3_aws__N12_cryptography__N8_keyStore__S15_VersionKeyInput__M19_branchKeyIdentifier(Dafny.ISequence<char> value)
     {
       return FromDafny_N6_smithy__N3_api__S6_String(value);
@@ -1181,21 +1270,13 @@ namespace AWS.Cryptography.KeyStore
     {
       return ToDafny_N6_smithy__N3_api__S6_String(value);
     }
-    public static AWS.Cryptography.KeyStore.EncryptedHierarchicalKey FromDafny_N3_aws__N12_cryptography__N8_keyStore__S28_WriteInitializeMutationInput__M6_Active(software.amazon.cryptography.keystore.internaldafny.types._IEncryptedHierarchicalKey value)
+    public static AWS.Cryptography.KeyStore.OverWriteEncryptedHierarchicalKey FromDafny_N3_aws__N12_cryptography__N8_keyStore__S28_WriteInitializeMutationInput__M6_Active(software.amazon.cryptography.keystore.internaldafny.types._IOverWriteEncryptedHierarchicalKey value)
     {
-      return FromDafny_N3_aws__N12_cryptography__N8_keyStore__S24_EncryptedHierarchicalKey(value);
+      return FromDafny_N3_aws__N12_cryptography__N8_keyStore__S33_OverWriteEncryptedHierarchicalKey(value);
     }
-    public static software.amazon.cryptography.keystore.internaldafny.types._IEncryptedHierarchicalKey ToDafny_N3_aws__N12_cryptography__N8_keyStore__S28_WriteInitializeMutationInput__M6_Active(AWS.Cryptography.KeyStore.EncryptedHierarchicalKey value)
+    public static software.amazon.cryptography.keystore.internaldafny.types._IOverWriteEncryptedHierarchicalKey ToDafny_N3_aws__N12_cryptography__N8_keyStore__S28_WriteInitializeMutationInput__M6_Active(AWS.Cryptography.KeyStore.OverWriteEncryptedHierarchicalKey value)
     {
-      return ToDafny_N3_aws__N12_cryptography__N8_keyStore__S24_EncryptedHierarchicalKey(value);
-    }
-    public static AWS.Cryptography.KeyStore.EncryptedHierarchicalKey FromDafny_N3_aws__N12_cryptography__N8_keyStore__S28_WriteInitializeMutationInput__M9_OldActive(software.amazon.cryptography.keystore.internaldafny.types._IEncryptedHierarchicalKey value)
-    {
-      return FromDafny_N3_aws__N12_cryptography__N8_keyStore__S24_EncryptedHierarchicalKey(value);
-    }
-    public static software.amazon.cryptography.keystore.internaldafny.types._IEncryptedHierarchicalKey ToDafny_N3_aws__N12_cryptography__N8_keyStore__S28_WriteInitializeMutationInput__M9_OldActive(AWS.Cryptography.KeyStore.EncryptedHierarchicalKey value)
-    {
-      return ToDafny_N3_aws__N12_cryptography__N8_keyStore__S24_EncryptedHierarchicalKey(value);
+      return ToDafny_N3_aws__N12_cryptography__N8_keyStore__S33_OverWriteEncryptedHierarchicalKey(value);
     }
     public static AWS.Cryptography.KeyStore.EncryptedHierarchicalKey FromDafny_N3_aws__N12_cryptography__N8_keyStore__S28_WriteInitializeMutationInput__M7_Version(software.amazon.cryptography.keystore.internaldafny.types._IEncryptedHierarchicalKey value)
     {
@@ -1205,13 +1286,13 @@ namespace AWS.Cryptography.KeyStore
     {
       return ToDafny_N3_aws__N12_cryptography__N8_keyStore__S24_EncryptedHierarchicalKey(value);
     }
-    public static AWS.Cryptography.KeyStore.EncryptedHierarchicalKey FromDafny_N3_aws__N12_cryptography__N8_keyStore__S28_WriteInitializeMutationInput__M6_Beacon(software.amazon.cryptography.keystore.internaldafny.types._IEncryptedHierarchicalKey value)
+    public static AWS.Cryptography.KeyStore.OverWriteEncryptedHierarchicalKey FromDafny_N3_aws__N12_cryptography__N8_keyStore__S28_WriteInitializeMutationInput__M6_Beacon(software.amazon.cryptography.keystore.internaldafny.types._IOverWriteEncryptedHierarchicalKey value)
     {
-      return FromDafny_N3_aws__N12_cryptography__N8_keyStore__S24_EncryptedHierarchicalKey(value);
+      return FromDafny_N3_aws__N12_cryptography__N8_keyStore__S33_OverWriteEncryptedHierarchicalKey(value);
     }
-    public static software.amazon.cryptography.keystore.internaldafny.types._IEncryptedHierarchicalKey ToDafny_N3_aws__N12_cryptography__N8_keyStore__S28_WriteInitializeMutationInput__M6_Beacon(AWS.Cryptography.KeyStore.EncryptedHierarchicalKey value)
+    public static software.amazon.cryptography.keystore.internaldafny.types._IOverWriteEncryptedHierarchicalKey ToDafny_N3_aws__N12_cryptography__N8_keyStore__S28_WriteInitializeMutationInput__M6_Beacon(AWS.Cryptography.KeyStore.OverWriteEncryptedHierarchicalKey value)
     {
-      return ToDafny_N3_aws__N12_cryptography__N8_keyStore__S24_EncryptedHierarchicalKey(value);
+      return ToDafny_N3_aws__N12_cryptography__N8_keyStore__S33_OverWriteEncryptedHierarchicalKey(value);
     }
     public static AWS.Cryptography.KeyStore.MutationLock FromDafny_N3_aws__N12_cryptography__N8_keyStore__S28_WriteInitializeMutationInput__M12_MutationLock(software.amazon.cryptography.keystore.internaldafny.types._IMutationLock value)
     {
@@ -1221,45 +1302,29 @@ namespace AWS.Cryptography.KeyStore
     {
       return ToDafny_N3_aws__N12_cryptography__N8_keyStore__S12_MutationLock(value);
     }
-    public static System.Collections.Generic.List<AWS.Cryptography.KeyStore.EncryptedHierarchicalKey> FromDafny_N3_aws__N12_cryptography__N8_keyStore__S25_WriteMutatedVersionsInput__M5_Items(Dafny.ISequence<software.amazon.cryptography.keystore.internaldafny.types._IEncryptedHierarchicalKey> value)
+    public static AWS.Cryptography.KeyStore.MutationIndex FromDafny_N3_aws__N12_cryptography__N8_keyStore__S28_WriteInitializeMutationInput__M13_MutationIndex(software.amazon.cryptography.keystore.internaldafny.types._IMutationIndex value)
     {
-      return FromDafny_N3_aws__N12_cryptography__N8_keyStore__S25_EncryptedHierarchicalKeys(value);
+      return FromDafny_N3_aws__N12_cryptography__N8_keyStore__S13_MutationIndex(value);
     }
-    public static Dafny.ISequence<software.amazon.cryptography.keystore.internaldafny.types._IEncryptedHierarchicalKey> ToDafny_N3_aws__N12_cryptography__N8_keyStore__S25_WriteMutatedVersionsInput__M5_Items(System.Collections.Generic.List<AWS.Cryptography.KeyStore.EncryptedHierarchicalKey> value)
+    public static software.amazon.cryptography.keystore.internaldafny.types._IMutationIndex ToDafny_N3_aws__N12_cryptography__N8_keyStore__S28_WriteInitializeMutationInput__M13_MutationIndex(AWS.Cryptography.KeyStore.MutationIndex value)
     {
-      return ToDafny_N3_aws__N12_cryptography__N8_keyStore__S25_EncryptedHierarchicalKeys(value);
+      return ToDafny_N3_aws__N12_cryptography__N8_keyStore__S13_MutationIndex(value);
     }
-    public static string FromDafny_N3_aws__N12_cryptography__N8_keyStore__S25_WriteMutatedVersionsInput__M10_Identifier(Dafny.ISequence<char> value)
+    public static System.Collections.Generic.List<AWS.Cryptography.KeyStore.OverWriteEncryptedHierarchicalKey> FromDafny_N3_aws__N12_cryptography__N8_keyStore__S25_WriteMutatedVersionsInput__M5_Items(Dafny.ISequence<software.amazon.cryptography.keystore.internaldafny.types._IOverWriteEncryptedHierarchicalKey> value)
     {
-      return FromDafny_N6_smithy__N3_api__S6_String(value);
+      return FromDafny_N3_aws__N12_cryptography__N8_keyStore__S34_OverWriteEncryptedHierarchicalKeys(value);
     }
-    public static Dafny.ISequence<char> ToDafny_N3_aws__N12_cryptography__N8_keyStore__S25_WriteMutatedVersionsInput__M10_Identifier(string value)
+    public static Dafny.ISequence<software.amazon.cryptography.keystore.internaldafny.types._IOverWriteEncryptedHierarchicalKey> ToDafny_N3_aws__N12_cryptography__N8_keyStore__S25_WriteMutatedVersionsInput__M5_Items(System.Collections.Generic.List<AWS.Cryptography.KeyStore.OverWriteEncryptedHierarchicalKey> value)
     {
-      return ToDafny_N6_smithy__N3_api__S6_String(value);
+      return ToDafny_N3_aws__N12_cryptography__N8_keyStore__S34_OverWriteEncryptedHierarchicalKeys(value);
     }
-    public static System.IO.MemoryStream FromDafny_N3_aws__N12_cryptography__N8_keyStore__S25_WriteMutatedVersionsInput__M8_Original(Dafny.ISequence<byte> value)
+    public static AWS.Cryptography.KeyStore.MutationLock FromDafny_N3_aws__N12_cryptography__N8_keyStore__S25_WriteMutatedVersionsInput__M12_MutationLock(software.amazon.cryptography.keystore.internaldafny.types._IMutationLock value)
     {
-      return FromDafny_N6_smithy__N3_api__S4_Blob(value);
+      return FromDafny_N3_aws__N12_cryptography__N8_keyStore__S12_MutationLock(value);
     }
-    public static Dafny.ISequence<byte> ToDafny_N3_aws__N12_cryptography__N8_keyStore__S25_WriteMutatedVersionsInput__M8_Original(System.IO.MemoryStream value)
+    public static software.amazon.cryptography.keystore.internaldafny.types._IMutationLock ToDafny_N3_aws__N12_cryptography__N8_keyStore__S25_WriteMutatedVersionsInput__M12_MutationLock(AWS.Cryptography.KeyStore.MutationLock value)
     {
-      return ToDafny_N6_smithy__N3_api__S4_Blob(value);
-    }
-    public static System.IO.MemoryStream FromDafny_N3_aws__N12_cryptography__N8_keyStore__S25_WriteMutatedVersionsInput__M8_Terminal(Dafny.ISequence<byte> value)
-    {
-      return FromDafny_N6_smithy__N3_api__S4_Blob(value);
-    }
-    public static Dafny.ISequence<byte> ToDafny_N3_aws__N12_cryptography__N8_keyStore__S25_WriteMutatedVersionsInput__M8_Terminal(System.IO.MemoryStream value)
-    {
-      return ToDafny_N6_smithy__N3_api__S4_Blob(value);
-    }
-    public static bool FromDafny_N3_aws__N12_cryptography__N8_keyStore__S25_WriteMutatedVersionsInput__M16_CompleteMutation(bool value)
-    {
-      return FromDafny_N6_smithy__N3_api__S7_Boolean(value);
-    }
-    public static bool ToDafny_N3_aws__N12_cryptography__N8_keyStore__S25_WriteMutatedVersionsInput__M16_CompleteMutation(bool value)
-    {
-      return ToDafny_N6_smithy__N3_api__S7_Boolean(value);
+      return ToDafny_N3_aws__N12_cryptography__N8_keyStore__S12_MutationLock(value);
     }
     public static AWS.Cryptography.KeyStore.EncryptedHierarchicalKey FromDafny_N3_aws__N12_cryptography__N8_keyStore__S31_WriteNewEncryptedBranchKeyInput__M6_Active(software.amazon.cryptography.keystore.internaldafny.types._IEncryptedHierarchicalKey value)
     {
@@ -1285,27 +1350,19 @@ namespace AWS.Cryptography.KeyStore
     {
       return ToDafny_N3_aws__N12_cryptography__N8_keyStore__S24_EncryptedHierarchicalKey(value);
     }
-    public static AWS.Cryptography.KeyStore.EncryptedHierarchicalKey FromDafny_N3_aws__N12_cryptography__N8_keyStore__S38_WriteNewEncryptedBranchKeyVersionInput__M6_Active(software.amazon.cryptography.keystore.internaldafny.types._IEncryptedHierarchicalKey value)
+    public static AWS.Cryptography.KeyStore.OverWriteEncryptedHierarchicalKey FromDafny_N3_aws__N12_cryptography__N8_keyStore__S38_WriteNewEncryptedBranchKeyVersionInput__M6_Active(software.amazon.cryptography.keystore.internaldafny.types._IOverWriteEncryptedHierarchicalKey value)
     {
-      return FromDafny_N3_aws__N12_cryptography__N8_keyStore__S24_EncryptedHierarchicalKey(value);
+      return FromDafny_N3_aws__N12_cryptography__N8_keyStore__S33_OverWriteEncryptedHierarchicalKey(value);
     }
-    public static software.amazon.cryptography.keystore.internaldafny.types._IEncryptedHierarchicalKey ToDafny_N3_aws__N12_cryptography__N8_keyStore__S38_WriteNewEncryptedBranchKeyVersionInput__M6_Active(AWS.Cryptography.KeyStore.EncryptedHierarchicalKey value)
+    public static software.amazon.cryptography.keystore.internaldafny.types._IOverWriteEncryptedHierarchicalKey ToDafny_N3_aws__N12_cryptography__N8_keyStore__S38_WriteNewEncryptedBranchKeyVersionInput__M6_Active(AWS.Cryptography.KeyStore.OverWriteEncryptedHierarchicalKey value)
     {
-      return ToDafny_N3_aws__N12_cryptography__N8_keyStore__S24_EncryptedHierarchicalKey(value);
+      return ToDafny_N3_aws__N12_cryptography__N8_keyStore__S33_OverWriteEncryptedHierarchicalKey(value);
     }
     public static AWS.Cryptography.KeyStore.EncryptedHierarchicalKey FromDafny_N3_aws__N12_cryptography__N8_keyStore__S38_WriteNewEncryptedBranchKeyVersionInput__M7_Version(software.amazon.cryptography.keystore.internaldafny.types._IEncryptedHierarchicalKey value)
     {
       return FromDafny_N3_aws__N12_cryptography__N8_keyStore__S24_EncryptedHierarchicalKey(value);
     }
     public static software.amazon.cryptography.keystore.internaldafny.types._IEncryptedHierarchicalKey ToDafny_N3_aws__N12_cryptography__N8_keyStore__S38_WriteNewEncryptedBranchKeyVersionInput__M7_Version(AWS.Cryptography.KeyStore.EncryptedHierarchicalKey value)
-    {
-      return ToDafny_N3_aws__N12_cryptography__N8_keyStore__S24_EncryptedHierarchicalKey(value);
-    }
-    public static AWS.Cryptography.KeyStore.EncryptedHierarchicalKey FromDafny_N3_aws__N12_cryptography__N8_keyStore__S38_WriteNewEncryptedBranchKeyVersionInput__M9_OldActive(software.amazon.cryptography.keystore.internaldafny.types._IEncryptedHierarchicalKey value)
-    {
-      return FromDafny_N3_aws__N12_cryptography__N8_keyStore__S24_EncryptedHierarchicalKey(value);
-    }
-    public static software.amazon.cryptography.keystore.internaldafny.types._IEncryptedHierarchicalKey ToDafny_N3_aws__N12_cryptography__N8_keyStore__S38_WriteNewEncryptedBranchKeyVersionInput__M9_OldActive(AWS.Cryptography.KeyStore.EncryptedHierarchicalKey value)
     {
       return ToDafny_N3_aws__N12_cryptography__N8_keyStore__S24_EncryptedHierarchicalKey(value);
     }
@@ -1316,20 +1373,6 @@ namespace AWS.Cryptography.KeyStore
     public static Dafny.ISequence<char> ToDafny_N6_smithy__N3_api__S6_String(string value)
     {
       return Dafny.Sequence<char>.FromString(value);
-    }
-    public static AWS.Cryptography.KeyStore.MutationLock FromDafny_N3_aws__N12_cryptography__N8_keyStore__S12_MutationLock(software.amazon.cryptography.keystore.internaldafny.types._IMutationLock value)
-    {
-      software.amazon.cryptography.keystore.internaldafny.types.MutationLock concrete = (software.amazon.cryptography.keystore.internaldafny.types.MutationLock)value; AWS.Cryptography.KeyStore.MutationLock converted = new AWS.Cryptography.KeyStore.MutationLock(); converted.Identifier = (string)FromDafny_N3_aws__N12_cryptography__N8_keyStore__S12_MutationLock__M10_Identifier(concrete._Identifier);
-      converted.CreateTime = (string)FromDafny_N3_aws__N12_cryptography__N8_keyStore__S12_MutationLock__M10_CreateTime(concrete._CreateTime);
-      converted.UUID = (string)FromDafny_N3_aws__N12_cryptography__N8_keyStore__S12_MutationLock__M4_UUID(concrete._UUID);
-      converted.Original = (System.IO.MemoryStream)FromDafny_N3_aws__N12_cryptography__N8_keyStore__S12_MutationLock__M8_Original(concrete._Original);
-      converted.Terminal = (System.IO.MemoryStream)FromDafny_N3_aws__N12_cryptography__N8_keyStore__S12_MutationLock__M8_Terminal(concrete._Terminal); return converted;
-    }
-    public static software.amazon.cryptography.keystore.internaldafny.types._IMutationLock ToDafny_N3_aws__N12_cryptography__N8_keyStore__S12_MutationLock(AWS.Cryptography.KeyStore.MutationLock value)
-    {
-      value.Validate();
-
-      return new software.amazon.cryptography.keystore.internaldafny.types.MutationLock(ToDafny_N3_aws__N12_cryptography__N8_keyStore__S12_MutationLock__M10_Identifier(value.Identifier), ToDafny_N3_aws__N12_cryptography__N8_keyStore__S12_MutationLock__M10_CreateTime(value.CreateTime), ToDafny_N3_aws__N12_cryptography__N8_keyStore__S12_MutationLock__M4_UUID(value.UUID), ToDafny_N3_aws__N12_cryptography__N8_keyStore__S12_MutationLock__M8_Original(value.Original), ToDafny_N3_aws__N12_cryptography__N8_keyStore__S12_MutationLock__M8_Terminal(value.Terminal));
     }
     public static System.Collections.Generic.Dictionary<string, string> FromDafny_N3_aws__N12_cryptography__N8_keyStore__S17_EncryptionContext(Dafny.IMap<Dafny.ISequence<byte>, Dafny.ISequence<byte>> value)
     {
@@ -1348,6 +1391,21 @@ namespace AWS.Cryptography.KeyStore
     public static Dafny.ISequence<char> ToDafny_N3_com__N9_amazonaws__N8_dynamodb__S8_TableArn(string value)
     {
       return Dafny.Sequence<char>.FromString(value);
+    }
+    public static AWS.Cryptography.KeyStore.MutationLock FromDafny_N3_aws__N12_cryptography__N8_keyStore__S12_MutationLock(software.amazon.cryptography.keystore.internaldafny.types._IMutationLock value)
+    {
+      software.amazon.cryptography.keystore.internaldafny.types.MutationLock concrete = (software.amazon.cryptography.keystore.internaldafny.types.MutationLock)value; AWS.Cryptography.KeyStore.MutationLock converted = new AWS.Cryptography.KeyStore.MutationLock(); converted.Identifier = (string)FromDafny_N3_aws__N12_cryptography__N8_keyStore__S12_MutationLock__M10_Identifier(concrete._Identifier);
+      converted.CreateTime = (string)FromDafny_N3_aws__N12_cryptography__N8_keyStore__S12_MutationLock__M10_CreateTime(concrete._CreateTime);
+      converted.UUID = (string)FromDafny_N3_aws__N12_cryptography__N8_keyStore__S12_MutationLock__M4_UUID(concrete._UUID);
+      converted.Original = (System.IO.MemoryStream)FromDafny_N3_aws__N12_cryptography__N8_keyStore__S12_MutationLock__M8_Original(concrete._Original);
+      converted.Terminal = (System.IO.MemoryStream)FromDafny_N3_aws__N12_cryptography__N8_keyStore__S12_MutationLock__M8_Terminal(concrete._Terminal);
+      converted.Enc = (System.IO.MemoryStream)FromDafny_N3_aws__N12_cryptography__N8_keyStore__S12_MutationLock__M3_Enc(concrete._Enc); return converted;
+    }
+    public static software.amazon.cryptography.keystore.internaldafny.types._IMutationLock ToDafny_N3_aws__N12_cryptography__N8_keyStore__S12_MutationLock(AWS.Cryptography.KeyStore.MutationLock value)
+    {
+      value.Validate();
+
+      return new software.amazon.cryptography.keystore.internaldafny.types.MutationLock(ToDafny_N3_aws__N12_cryptography__N8_keyStore__S12_MutationLock__M10_Identifier(value.Identifier), ToDafny_N3_aws__N12_cryptography__N8_keyStore__S12_MutationLock__M10_CreateTime(value.CreateTime), ToDafny_N3_aws__N12_cryptography__N8_keyStore__S12_MutationLock__M4_UUID(value.UUID), ToDafny_N3_aws__N12_cryptography__N8_keyStore__S12_MutationLock__M8_Original(value.Original), ToDafny_N3_aws__N12_cryptography__N8_keyStore__S12_MutationLock__M8_Terminal(value.Terminal), ToDafny_N3_aws__N12_cryptography__N8_keyStore__S12_MutationLock__M3_Enc(value.Enc));
     }
     public static AWS.Cryptography.KeyStore.BranchKeyMaterials FromDafny_N3_aws__N12_cryptography__N8_keyStore__S18_BranchKeyMaterials(software.amazon.cryptography.keystore.internaldafny.types._IBranchKeyMaterials value)
     {
@@ -1390,6 +1448,20 @@ namespace AWS.Cryptography.KeyStore
       value.Validate();
 
       return new software.amazon.cryptography.keystore.internaldafny.types.EncryptedHierarchicalKey(ToDafny_N3_aws__N12_cryptography__N8_keyStore__S24_EncryptedHierarchicalKey__M10_Identifier(value.Identifier), ToDafny_N3_aws__N12_cryptography__N8_keyStore__S24_EncryptedHierarchicalKey__M4_Type(value.Type), ToDafny_N3_aws__N12_cryptography__N8_keyStore__S24_EncryptedHierarchicalKey__M10_CreateTime(value.CreateTime), ToDafny_N3_aws__N12_cryptography__N8_keyStore__S24_EncryptedHierarchicalKey__M6_KmsArn(value.KmsArn), ToDafny_N3_aws__N12_cryptography__N8_keyStore__S24_EncryptedHierarchicalKey__M17_EncryptionContext(value.EncryptionContext), ToDafny_N3_aws__N12_cryptography__N8_keyStore__S24_EncryptedHierarchicalKey__M14_CiphertextBlob(value.CiphertextBlob));
+    }
+    public static AWS.Cryptography.KeyStore.MutationIndex FromDafny_N3_aws__N12_cryptography__N8_keyStore__S13_MutationIndex(software.amazon.cryptography.keystore.internaldafny.types._IMutationIndex value)
+    {
+      software.amazon.cryptography.keystore.internaldafny.types.MutationIndex concrete = (software.amazon.cryptography.keystore.internaldafny.types.MutationIndex)value; AWS.Cryptography.KeyStore.MutationIndex converted = new AWS.Cryptography.KeyStore.MutationIndex(); converted.Identifier = (string)FromDafny_N3_aws__N12_cryptography__N8_keyStore__S13_MutationIndex__M10_Identifier(concrete._Identifier);
+      converted.CreateTime = (string)FromDafny_N3_aws__N12_cryptography__N8_keyStore__S13_MutationIndex__M10_CreateTime(concrete._CreateTime);
+      converted.UUID = (string)FromDafny_N3_aws__N12_cryptography__N8_keyStore__S13_MutationIndex__M4_UUID(concrete._UUID);
+      converted.PageIndex = (System.IO.MemoryStream)FromDafny_N3_aws__N12_cryptography__N8_keyStore__S13_MutationIndex__M9_PageIndex(concrete._PageIndex);
+      converted.Enc = (System.IO.MemoryStream)FromDafny_N3_aws__N12_cryptography__N8_keyStore__S13_MutationIndex__M3_Enc(concrete._Enc); return converted;
+    }
+    public static software.amazon.cryptography.keystore.internaldafny.types._IMutationIndex ToDafny_N3_aws__N12_cryptography__N8_keyStore__S13_MutationIndex(AWS.Cryptography.KeyStore.MutationIndex value)
+    {
+      value.Validate();
+
+      return new software.amazon.cryptography.keystore.internaldafny.types.MutationIndex(ToDafny_N3_aws__N12_cryptography__N8_keyStore__S13_MutationIndex__M10_Identifier(value.Identifier), ToDafny_N3_aws__N12_cryptography__N8_keyStore__S13_MutationIndex__M10_CreateTime(value.CreateTime), ToDafny_N3_aws__N12_cryptography__N8_keyStore__S13_MutationIndex__M4_UUID(value.UUID), ToDafny_N3_aws__N12_cryptography__N8_keyStore__S13_MutationIndex__M9_PageIndex(value.PageIndex), ToDafny_N3_aws__N12_cryptography__N8_keyStore__S13_MutationIndex__M3_Enc(value.Enc));
     }
     public static string FromDafny_N3_aws__N12_cryptography__N8_keyStore__S9_Utf8Bytes(Dafny.ISequence<byte> value)
     {
@@ -1566,13 +1638,40 @@ namespace AWS.Cryptography.KeyStore
               "Custom implementations of KeyStorageInterface must extend KeyStorageInterfaceBase.");
       }
     }
-    public static bool FromDafny_N6_smithy__N3_api__S7_Boolean(bool value)
+    public static AWS.Cryptography.KeyStore.OverWriteEncryptedHierarchicalKey FromDafny_N3_aws__N12_cryptography__N8_keyStore__S33_OverWriteEncryptedHierarchicalKey(software.amazon.cryptography.keystore.internaldafny.types._IOverWriteEncryptedHierarchicalKey value)
     {
-      return value;
+      software.amazon.cryptography.keystore.internaldafny.types.OverWriteEncryptedHierarchicalKey concrete = (software.amazon.cryptography.keystore.internaldafny.types.OverWriteEncryptedHierarchicalKey)value; AWS.Cryptography.KeyStore.OverWriteEncryptedHierarchicalKey converted = new AWS.Cryptography.KeyStore.OverWriteEncryptedHierarchicalKey(); converted.EncryptedHierarchicalKey = (AWS.Cryptography.KeyStore.EncryptedHierarchicalKey)FromDafny_N3_aws__N12_cryptography__N8_keyStore__S33_OverWriteEncryptedHierarchicalKey__M24_EncryptedHierarchicalKey(concrete._EncryptedHierarchicalKey);
+      converted.Old = (AWS.Cryptography.KeyStore.EncryptedHierarchicalKey)FromDafny_N3_aws__N12_cryptography__N8_keyStore__S33_OverWriteEncryptedHierarchicalKey__M3_Old(concrete._Old); return converted;
     }
-    public static bool ToDafny_N6_smithy__N3_api__S7_Boolean(bool value)
+    public static software.amazon.cryptography.keystore.internaldafny.types._IOverWriteEncryptedHierarchicalKey ToDafny_N3_aws__N12_cryptography__N8_keyStore__S33_OverWriteEncryptedHierarchicalKey(AWS.Cryptography.KeyStore.OverWriteEncryptedHierarchicalKey value)
     {
-      return value;
+      value.Validate();
+
+      return new software.amazon.cryptography.keystore.internaldafny.types.OverWriteEncryptedHierarchicalKey(ToDafny_N3_aws__N12_cryptography__N8_keyStore__S33_OverWriteEncryptedHierarchicalKey__M24_EncryptedHierarchicalKey(value.EncryptedHierarchicalKey), ToDafny_N3_aws__N12_cryptography__N8_keyStore__S33_OverWriteEncryptedHierarchicalKey__M3_Old(value.Old));
+    }
+    public static System.Collections.Generic.List<AWS.Cryptography.KeyStore.OverWriteEncryptedHierarchicalKey> FromDafny_N3_aws__N12_cryptography__N8_keyStore__S34_OverWriteEncryptedHierarchicalKeys(Dafny.ISequence<software.amazon.cryptography.keystore.internaldafny.types._IOverWriteEncryptedHierarchicalKey> value)
+    {
+      return new System.Collections.Generic.List<AWS.Cryptography.KeyStore.OverWriteEncryptedHierarchicalKey>(value.Elements.Select(FromDafny_N3_aws__N12_cryptography__N8_keyStore__S34_OverWriteEncryptedHierarchicalKeys__M6_member));
+    }
+    public static Dafny.ISequence<software.amazon.cryptography.keystore.internaldafny.types._IOverWriteEncryptedHierarchicalKey> ToDafny_N3_aws__N12_cryptography__N8_keyStore__S34_OverWriteEncryptedHierarchicalKeys(System.Collections.Generic.List<AWS.Cryptography.KeyStore.OverWriteEncryptedHierarchicalKey> value)
+    {
+      return Dafny.Sequence<software.amazon.cryptography.keystore.internaldafny.types._IOverWriteEncryptedHierarchicalKey>.FromArray(value.Select(ToDafny_N3_aws__N12_cryptography__N8_keyStore__S34_OverWriteEncryptedHierarchicalKeys__M6_member).ToArray());
+    }
+    public static string FromDafny_N3_aws__N12_cryptography__N8_keyStore__S17_EncryptionContext__M3_key(Dafny.ISequence<byte> value)
+    {
+      return FromDafny_N3_aws__N12_cryptography__N8_keyStore__S9_Utf8Bytes(value);
+    }
+    public static Dafny.ISequence<byte> ToDafny_N3_aws__N12_cryptography__N8_keyStore__S17_EncryptionContext__M3_key(string value)
+    {
+      return ToDafny_N3_aws__N12_cryptography__N8_keyStore__S9_Utf8Bytes(value);
+    }
+    public static string FromDafny_N3_aws__N12_cryptography__N8_keyStore__S17_EncryptionContext__M5_value(Dafny.ISequence<byte> value)
+    {
+      return FromDafny_N3_aws__N12_cryptography__N8_keyStore__S9_Utf8Bytes(value);
+    }
+    public static Dafny.ISequence<byte> ToDafny_N3_aws__N12_cryptography__N8_keyStore__S17_EncryptionContext__M5_value(string value)
+    {
+      return ToDafny_N3_aws__N12_cryptography__N8_keyStore__S9_Utf8Bytes(value);
     }
     public static string FromDafny_N3_aws__N12_cryptography__N8_keyStore__S12_MutationLock__M10_Identifier(Dafny.ISequence<char> value)
     {
@@ -1614,21 +1713,13 @@ namespace AWS.Cryptography.KeyStore
     {
       return ToDafny_N6_smithy__N3_api__S4_Blob(value);
     }
-    public static string FromDafny_N3_aws__N12_cryptography__N8_keyStore__S17_EncryptionContext__M3_key(Dafny.ISequence<byte> value)
+    public static System.IO.MemoryStream FromDafny_N3_aws__N12_cryptography__N8_keyStore__S12_MutationLock__M3_Enc(Dafny.ISequence<byte> value)
     {
-      return FromDafny_N3_aws__N12_cryptography__N8_keyStore__S9_Utf8Bytes(value);
+      return FromDafny_N6_smithy__N3_api__S4_Blob(value);
     }
-    public static Dafny.ISequence<byte> ToDafny_N3_aws__N12_cryptography__N8_keyStore__S17_EncryptionContext__M3_key(string value)
+    public static Dafny.ISequence<byte> ToDafny_N3_aws__N12_cryptography__N8_keyStore__S12_MutationLock__M3_Enc(System.IO.MemoryStream value)
     {
-      return ToDafny_N3_aws__N12_cryptography__N8_keyStore__S9_Utf8Bytes(value);
-    }
-    public static string FromDafny_N3_aws__N12_cryptography__N8_keyStore__S17_EncryptionContext__M5_value(Dafny.ISequence<byte> value)
-    {
-      return FromDafny_N3_aws__N12_cryptography__N8_keyStore__S9_Utf8Bytes(value);
-    }
-    public static Dafny.ISequence<byte> ToDafny_N3_aws__N12_cryptography__N8_keyStore__S17_EncryptionContext__M5_value(string value)
-    {
-      return ToDafny_N3_aws__N12_cryptography__N8_keyStore__S9_Utf8Bytes(value);
+      return ToDafny_N6_smithy__N3_api__S4_Blob(value);
     }
     public static string FromDafny_N3_aws__N12_cryptography__N8_keyStore__S18_BranchKeyMaterials__M19_branchKeyIdentifier(Dafny.ISequence<char> value)
     {
@@ -1742,6 +1833,46 @@ namespace AWS.Cryptography.KeyStore
     {
       return ToDafny_N6_smithy__N3_api__S4_Blob(value);
     }
+    public static string FromDafny_N3_aws__N12_cryptography__N8_keyStore__S13_MutationIndex__M10_Identifier(Dafny.ISequence<char> value)
+    {
+      return FromDafny_N6_smithy__N3_api__S6_String(value);
+    }
+    public static Dafny.ISequence<char> ToDafny_N3_aws__N12_cryptography__N8_keyStore__S13_MutationIndex__M10_Identifier(string value)
+    {
+      return ToDafny_N6_smithy__N3_api__S6_String(value);
+    }
+    public static string FromDafny_N3_aws__N12_cryptography__N8_keyStore__S13_MutationIndex__M10_CreateTime(Dafny.ISequence<char> value)
+    {
+      return FromDafny_N6_smithy__N3_api__S6_String(value);
+    }
+    public static Dafny.ISequence<char> ToDafny_N3_aws__N12_cryptography__N8_keyStore__S13_MutationIndex__M10_CreateTime(string value)
+    {
+      return ToDafny_N6_smithy__N3_api__S6_String(value);
+    }
+    public static string FromDafny_N3_aws__N12_cryptography__N8_keyStore__S13_MutationIndex__M4_UUID(Dafny.ISequence<char> value)
+    {
+      return FromDafny_N6_smithy__N3_api__S6_String(value);
+    }
+    public static Dafny.ISequence<char> ToDafny_N3_aws__N12_cryptography__N8_keyStore__S13_MutationIndex__M4_UUID(string value)
+    {
+      return ToDafny_N6_smithy__N3_api__S6_String(value);
+    }
+    public static System.IO.MemoryStream FromDafny_N3_aws__N12_cryptography__N8_keyStore__S13_MutationIndex__M9_PageIndex(Dafny.ISequence<byte> value)
+    {
+      return FromDafny_N6_smithy__N3_api__S4_Blob(value);
+    }
+    public static Dafny.ISequence<byte> ToDafny_N3_aws__N12_cryptography__N8_keyStore__S13_MutationIndex__M9_PageIndex(System.IO.MemoryStream value)
+    {
+      return ToDafny_N6_smithy__N3_api__S4_Blob(value);
+    }
+    public static System.IO.MemoryStream FromDafny_N3_aws__N12_cryptography__N8_keyStore__S13_MutationIndex__M3_Enc(Dafny.ISequence<byte> value)
+    {
+      return FromDafny_N6_smithy__N3_api__S4_Blob(value);
+    }
+    public static Dafny.ISequence<byte> ToDafny_N3_aws__N12_cryptography__N8_keyStore__S13_MutationIndex__M3_Enc(System.IO.MemoryStream value)
+    {
+      return ToDafny_N6_smithy__N3_api__S4_Blob(value);
+    }
     public static string FromDafny_N3_aws__N12_cryptography__N8_keyStore__S14_GrantTokenList__M6_member(Dafny.ISequence<char> value)
     {
       return FromDafny_N6_smithy__N3_api__S6_String(value);
@@ -1813,6 +1944,30 @@ namespace AWS.Cryptography.KeyStore
     public static Wrappers_Compile._IOption<software.amazon.cryptography.services.dynamodb.internaldafny.types.IDynamoDBClient> ToDafny_N3_aws__N12_cryptography__N8_keyStore__S13_DynamoDBTable__M9_ddbClient(Amazon.DynamoDBv2.IAmazonDynamoDB value)
     {
       return value == null ? Wrappers_Compile.Option<software.amazon.cryptography.services.dynamodb.internaldafny.types.IDynamoDBClient>.create_None() : Wrappers_Compile.Option<software.amazon.cryptography.services.dynamodb.internaldafny.types.IDynamoDBClient>.create_Some(ToDafny_N3_aws__N12_cryptography__N8_keyStore__S18_DdbClientReference((Amazon.DynamoDBv2.IAmazonDynamoDB)value));
+    }
+    public static AWS.Cryptography.KeyStore.EncryptedHierarchicalKey FromDafny_N3_aws__N12_cryptography__N8_keyStore__S33_OverWriteEncryptedHierarchicalKey__M24_EncryptedHierarchicalKey(software.amazon.cryptography.keystore.internaldafny.types._IEncryptedHierarchicalKey value)
+    {
+      return FromDafny_N3_aws__N12_cryptography__N8_keyStore__S24_EncryptedHierarchicalKey(value);
+    }
+    public static software.amazon.cryptography.keystore.internaldafny.types._IEncryptedHierarchicalKey ToDafny_N3_aws__N12_cryptography__N8_keyStore__S33_OverWriteEncryptedHierarchicalKey__M24_EncryptedHierarchicalKey(AWS.Cryptography.KeyStore.EncryptedHierarchicalKey value)
+    {
+      return ToDafny_N3_aws__N12_cryptography__N8_keyStore__S24_EncryptedHierarchicalKey(value);
+    }
+    public static AWS.Cryptography.KeyStore.EncryptedHierarchicalKey FromDafny_N3_aws__N12_cryptography__N8_keyStore__S33_OverWriteEncryptedHierarchicalKey__M3_Old(software.amazon.cryptography.keystore.internaldafny.types._IEncryptedHierarchicalKey value)
+    {
+      return FromDafny_N3_aws__N12_cryptography__N8_keyStore__S24_EncryptedHierarchicalKey(value);
+    }
+    public static software.amazon.cryptography.keystore.internaldafny.types._IEncryptedHierarchicalKey ToDafny_N3_aws__N12_cryptography__N8_keyStore__S33_OverWriteEncryptedHierarchicalKey__M3_Old(AWS.Cryptography.KeyStore.EncryptedHierarchicalKey value)
+    {
+      return ToDafny_N3_aws__N12_cryptography__N8_keyStore__S24_EncryptedHierarchicalKey(value);
+    }
+    public static AWS.Cryptography.KeyStore.OverWriteEncryptedHierarchicalKey FromDafny_N3_aws__N12_cryptography__N8_keyStore__S34_OverWriteEncryptedHierarchicalKeys__M6_member(software.amazon.cryptography.keystore.internaldafny.types._IOverWriteEncryptedHierarchicalKey value)
+    {
+      return FromDafny_N3_aws__N12_cryptography__N8_keyStore__S33_OverWriteEncryptedHierarchicalKey(value);
+    }
+    public static software.amazon.cryptography.keystore.internaldafny.types._IOverWriteEncryptedHierarchicalKey ToDafny_N3_aws__N12_cryptography__N8_keyStore__S34_OverWriteEncryptedHierarchicalKeys__M6_member(AWS.Cryptography.KeyStore.OverWriteEncryptedHierarchicalKey value)
+    {
+      return ToDafny_N3_aws__N12_cryptography__N8_keyStore__S33_OverWriteEncryptedHierarchicalKey(value);
     }
     public static System.IO.MemoryStream FromDafny_N3_aws__N12_cryptography__N8_keyStore__S6_Secret(Dafny.ISequence<byte> value)
     {
