AwsCryptographicMaterialProviders/runtimes/net/Generated/AwsCryptographyKeyStoreAdmin/InitializeMutationFlag.cs
@@ -1,0 +1,51 @@
+// Copyright Amazon.com Inc. or its affiliates. All Rights Reserved.
+// SPDX-License-Identifier: Apache-2.0
+// Do not modify this file. This file is machine generated, and any changes to it will be overwritten.
+using System;
+using AWS.Cryptography.KeyStoreAdmin;
+namespace AWS.Cryptography.KeyStoreAdmin
+{
+  public class InitializeMutationFlag
+  {
+    private string _created;
+    private string _resumed;
+    private string _resumedWithoutIndex;
+    public string Created
+    {
+      get { return this._created; }
+      set { this._created = value; }
+    }
+    public bool IsSetCreated()
+    {
+      return this._created != null;
+    }
+    public string Resumed
+    {
+      get { return this._resumed; }
+      set { this._resumed = value; }
+    }
+    public bool IsSetResumed()
+    {
+      return this._resumed != null;
+    }
+    public string ResumedWithoutIndex
+    {
+      get { return this._resumedWithoutIndex; }
+      set { this._resumedWithoutIndex = value; }
+    }
+    public bool IsSetResumedWithoutIndex()
+    {
+      return this._resumedWithoutIndex != null;
+    }
+    public void Validate()
+    {
+      var numberOfPropertiesSet = Convert.ToUInt16(IsSetCreated()) +
+      Convert.ToUInt16(IsSetResumed()) +
+      Convert.ToUInt16(IsSetResumedWithoutIndex());
+      if (numberOfPropertiesSet == 0) throw new System.ArgumentException("No union value set");
+
+      if (numberOfPropertiesSet > 1) throw new System.ArgumentException("Multiple union values set");
+
+    }
+  }
+}
